src/HOL/MicroJava/Comp/LemmasComp.thy
@@ -8,8 +8,15 @@
 
 theory LemmasComp = TranslComp:
 
+
+declare split_paired_All [simp del]
+declare split_paired_Ex [simp del]
+
+
 (**********************************************************************)
 (* misc lemmas *)
+
+
 
 lemma split_pairs: "(\<lambda>(a,b). (F a b)) (ab) = F (fst ab) (snd ab)"
 proof -
@@ -34,6 +41,44 @@ lemma c_hupd_hp_invariant: "gh (c_hupd hp (None, st)) = hp"
 by (case_tac st, simp add: c_hupd_conv gh_def)
 
 
+lemma unique_map_fst [rule_format]: "(\<forall> x \<in> set xs. (fst x = fst (f x) )) \<longrightarrow>
+  unique (map f xs) = unique xs"
+proof (induct xs)
+  case Nil show ?case by simp
+next
+  case (Cons a list)
+  show ?case
+  proof
+    assume fst_eq: "\<forall>x\<in>set (a # list). fst x = fst (f x)"
+
+    have fst_set: "(fst a \<in> fst ` set list) = (fst (f a) \<in> fst ` f ` set list)" 
+    proof 
+      assume as: "fst a \<in> fst ` set list" 
+      then obtain x where fst_a_x: "x\<in>set list \<and> fst a = fst x" 
+	by (auto simp add: image_iff)
+      then have "fst (f a) = fst (f x)" by (simp add: fst_eq)
+      with as show "(fst (f a) \<in> fst ` f ` set list)" by (simp add: fst_a_x)
+    next
+      assume as: "fst (f a) \<in> fst ` f ` set list"
+      then obtain x where fst_a_x: "x\<in>set list \<and> fst (f a) = fst (f x)"
+	by (auto simp add: image_iff)
+      then have "fst a = fst x" by (simp add: fst_eq)
+      with as show "fst a \<in> fst ` set list" by (simp add: fst_a_x)
+    qed
+
+    with fst_eq Cons 
+    show "unique (map f (a # list)) = unique (a # list)"
+      by (simp add: unique_def fst_set)
+  qed
+qed
+
+lemma comp_unique: "unique (comp G) = unique G"
+apply (simp add: comp_def)
+apply (rule unique_map_fst)
+apply (simp add: compClass_def split_beta)
+done
+
+
 (**********************************************************************)
 (* invariance of properties under compilation *)
 
@@ -53,75 +98,96 @@ apply (simp add: map_of_in_set)
 apply (simp add: image_compose [THEN sym] o_def split_beta del: image_compose)
 done
 
-lemma comp_is_class: "is_class G C = is_class (comp G) C"
+lemma comp_is_class: "is_class (comp G) C = is_class G C"
 by (case_tac "class G C", auto simp: is_class_def comp_class_None dest: comp_class_imp)
 
 
-lemma comp_is_type: "is_type G T = is_type (comp G) T"
+lemma comp_is_type: "is_type (comp G) T = is_type G T"
   by ((cases T),simp,(induct G)) ((simp),(simp only: comp_is_class),(simp add: comp_is_class),(simp only: comp_is_class))
 
-lemma SIGMA_cong: "\<lbrakk> A = B; !!x. x \<in> B \<Longrightarrow> C x = D x \<rbrakk> \<Longrightarrow> (\<Sigma> x \<in> A. C x) = (\<Sigma> x \<in> B. D x)"
+lemma SIGMA_cong: "\<lbrakk> A = B; !!x. x \<in> B \<Longrightarrow> C x = D x \<rbrakk> 
+  \<Longrightarrow> (\<Sigma> x \<in> A. C x) = (\<Sigma> x \<in> B. D x)"
 by auto
 
-lemma comp_classname: "is_class G C \<Longrightarrow> fst (the (class G C)) = fst (the (class (comp G) C))"
+lemma comp_classname: "is_class G C 
+  \<Longrightarrow> fst (the (class G C)) = fst (the (class (comp G) C))"
 by (case_tac "class G C", auto simp: is_class_def dest: comp_class_imp)
 
 
-lemma comp_subcls1: "subcls1 G = subcls1 (comp G)"
+lemma comp_subcls1: "subcls1 (comp G) = subcls1 G"
 apply (simp add: subcls1_def2 comp_is_class)
 apply (rule SIGMA_cong, simp)
-apply (simp add: comp_is_class [THEN sym])
+apply (simp add: comp_is_class)
 apply (simp add: comp_classname)
 done
 
-lemma comp_subcls: "(subcls1 G)^* = (subcls1 (comp G))^*"
-  by (induct G) (simp_all add: comp_def comp_subcls1)
-
-lemma comp_widen: "((ty1,ty2) \<in> widen G) = ((ty1,ty2) \<in> widen (comp G))"
+lemma comp_widen: "((ty1,ty2) \<in> widen (comp G)) = ((ty1,ty2) \<in> widen G)"
   apply rule
-  apply (cases "(ty1,ty2)" G rule: widen.cases) 
-  apply (simp_all add: comp_subcls widen.null)
   apply (cases "(ty1,ty2)" "comp G" rule: widen.cases) 
-  apply (simp_all add: comp_subcls widen.null)
+  apply (simp_all add: comp_subcls1 widen.null)
+  apply (cases "(ty1,ty2)" G rule: widen.cases) 
+  apply (simp_all add: comp_subcls1 widen.null)
   done
 
-lemma comp_cast: "((ty1,ty2) \<in> cast G) = ((ty1,ty2) \<in> cast (comp G))"
+lemma comp_cast: "((ty1,ty2) \<in> cast (comp G)) = ((ty1,ty2) \<in> cast G)"
   apply rule
-  apply (cases "(ty1,ty2)" G rule: cast.cases)
-  apply (simp_all add: comp_subcls cast.widen cast.subcls)
   apply (cases "(ty1,ty2)" "comp G" rule: cast.cases) 
-  apply (simp_all add: comp_subcls cast.widen cast.subcls)
+  apply (simp_all add: comp_subcls1 cast.widen cast.subcls)
+  apply (rule cast.widen) apply (simp add: comp_widen)
+  apply (cases "(ty1,ty2)" G rule: cast.cases)
+  apply (simp_all add: comp_subcls1 cast.widen cast.subcls)
+  apply (rule cast.widen) apply (simp add: comp_widen)
   done
 
-lemma comp_cast_ok: "cast_ok G = cast_ok (comp G)"
+lemma comp_cast_ok: "cast_ok (comp G) = cast_ok G"
   by (simp add: expand_fun_eq cast_ok_def comp_widen)
 
 
-lemma comp_wf_fdecl: "wf_fdecl G fd  \<Longrightarrow> wf_fdecl (comp G) fd"
-apply (case_tac fd)
-apply (simp add: wf_fdecl_def comp_is_type)
+lemma compClass_fst [simp]: "(fst (compClass G C)) = (fst C)"
+by (simp add: compClass_def split_beta)
+
+lemma compClass_fst_snd [simp]: "(fst (snd (compClass G C))) = (fst (snd C))"
+by (simp add: compClass_def split_beta)
+
+lemma compClass_fst_snd_snd [simp]: "(fst (snd (snd (compClass G C)))) = (fst (snd (snd C)))"
+by (simp add: compClass_def split_beta)
+
+lemma comp_wf_fdecl [simp]: "wf_fdecl (comp G) fd = wf_fdecl G fd"
+by (case_tac fd, simp add: wf_fdecl_def comp_is_type)
+
+
+lemma compClass_forall [simp]: "
+  (\<forall>x\<in>set (snd (snd (snd (compClass G C)))). P (fst x) (fst (snd x))) =
+  (\<forall>x\<in>set (snd (snd (snd C))). P (fst x) (fst (snd x)))"
+by (simp add: compClass_def compMethod_def split_beta)
+
+lemma comp_wf_mhead: "wf_mhead (comp G) S rT =  wf_mhead G S rT"
+by (simp add: wf_mhead_def split_beta comp_is_type)
+
+lemma comp_ws_cdecl: "
+  ws_cdecl (TranslComp.comp G) (compClass G C) = ws_cdecl G C"
+apply (simp add: ws_cdecl_def split_beta comp_is_class comp_subcls1)
+apply (simp (no_asm_simp) add: comp_wf_mhead)
+apply (simp add: compClass_def compMethod_def split_beta unique_map_fst)
 done
 
-lemma comp_wf_syscls: "wf_syscls G = wf_syscls (comp G)"
+
+lemma comp_wf_syscls: "wf_syscls (comp G) = wf_syscls G"
 apply (simp add: wf_syscls_def comp_def compClass_def split_beta)
 apply (simp only: image_compose [THEN sym])
-apply (subgoal_tac "(Fun.comp fst (\<lambda>(C, cno::cname, fdls::fdecl list, jmdls). (C, cno, fdls, map (compMethod G C) jmdls))) = fst")
-(*
-apply (subgoal_tac "(fst o (\<lambda>(C, cno::cname, fdls::fdecl list, jmdls). (C, cno, fdls, map (compMethod G C) jmdls))) = fst")
-*)
+apply (subgoal_tac "(Fun.comp fst (\<lambda>(C, cno::cname, fdls::fdecl list, jmdls).
+  (C, cno, fdls, map (compMethod G C) jmdls))) = fst")
 apply (simp del: image_compose)
 apply (simp add: expand_fun_eq split_beta)
 done
 
 
-lemma comp_wf_mhead: "wf_mhead G S rT =  wf_mhead (comp G) S rT"
-by (simp add: wf_mhead_def split_beta comp_is_type)
-
-lemma comp_wf_mdecl: "\<lbrakk> wf_mdecl wf_mb G C jmdl;
-  (wf_mb G C jmdl) \<longrightarrow> (wf_mb_comp (comp G) C (compMethod G C jmdl)) \<rbrakk> 
- \<Longrightarrow> 
-  wf_mdecl wf_mb_comp (comp G) C (compMethod G C jmdl)"
-by (simp add: wf_mdecl_def wf_mhead_def comp_is_type split_beta compMethod_def)
+lemma comp_ws_prog: "ws_prog (comp G) = ws_prog G"
+apply (rule sym)
+apply (simp add: ws_prog_def comp_ws_cdecl comp_unique)
+apply (simp add: comp_wf_syscls)
+apply (auto simp add: comp_ws_cdecl [THEN sym] TranslComp.comp_def)
+done
 
 
 lemma comp_class_rec: " wf ((subcls1 G)^-1) \<Longrightarrow> 
@@ -159,16 +225,16 @@ apply (simp add: comp_subcls1)
 done
 
 lemma comp_fields: "wf ((subcls1 G)^-1) \<Longrightarrow> 
-  fields (G,C) = fields (comp G,C)" 
+  fields (comp G,C) = fields (G,C)" 
 by (simp add: fields_def comp_class_rec)
 
 lemma comp_field: "wf ((subcls1 G)^-1) \<Longrightarrow> 
-  field (G,C) = field (comp G,C)" 
+  field (comp G,C) = field (G,C)" 
 by (simp add: field_def comp_fields)
 
 
 
-lemma class_rec_relation [rule_format (no_asm)]: "\<lbrakk>  wf_prog wf_mb G;
+lemma class_rec_relation [rule_format (no_asm)]: "\<lbrakk>  ws_prog G;
   \<forall> fs ms. R (f1 Object fs ms t1) (f2 Object fs ms t2);
    \<forall> C fs ms r1 r2. (R r1 r2) \<longrightarrow> (R (f1 C fs ms r1) (f2 C fs ms r2)) \<rbrakk>
   \<Longrightarrow> ((class G C) \<noteq> None) \<longrightarrow> 
@@ -194,10 +260,11 @@ apply (case_tac "x = Object")
 
   (* subgoals *)
 
-apply (frule class_wf) apply assumption
-apply (simp add: wf_cdecl_def is_class_def)
+apply (frule class_wf_struct) apply assumption
+apply (simp add: ws_cdecl_def is_class_def)
 
 apply (simp add: subcls1_def2 is_class_def)
+apply auto
 done
 
 
@@ -206,189 +273,114 @@ syntax
 translations
   "mtd_mb" => "Fun.comp snd snd"
 
-
-lemma map_of_map_fst: "\<lbrakk> map_of (map f xs) k = Some e; inj f;
+lemma map_of_map_fst: "\<lbrakk> inj f;
   \<forall>x\<in>set xs. fst (f x) = fst x; \<forall>x\<in>set xs. fst (g x) = fst x \<rbrakk>
-  \<Longrightarrow>  map_of (map g xs) k = Some (snd (g ((inv f) (k, e))))"
+  \<Longrightarrow>  map_of (map g xs) k 
+  = option_map (\<lambda> e. (snd (g ((inv f) (k, e))))) (map_of (map f xs) k)"
 apply (induct xs)
 apply simp
 apply (simp del: split_paired_All)
 apply (case_tac "k = fst a")
 apply (simp del: split_paired_All)
-apply (subgoal_tac "(fst a, e)  = f a")
+apply (subgoal_tac "(inv f (fst a, snd (f a))) = a", simp)
+apply (subgoal_tac "(fst a, snd (f a)) = f a", simp)
+apply (erule conjE)+
+apply (drule_tac s ="fst (f a)" and t="fst a" in sym)
 apply simp
-apply (rule_tac s= "(fst (f a), snd (f a))" in trans)
-apply simp
-apply (rule surjective_pairing [THEN sym])
-apply (simp del: split_paired_All)
+apply (simp add: surjective_pairing)
 done
 
 
-lemma comp_method [rule_format (no_asm)]: "\<lbrakk> wf_prog wf_mb G; is_class G C\<rbrakk> \<Longrightarrow> 
-  (method (G, C) S) = Some (D, rT, mb) \<longrightarrow> 
-  (method (comp G, C) S) = Some (D, rT, mtd_mb (compMethod G D (S, rT, mb)))"
+lemma comp_method [rule_format (no_asm)]: "\<lbrakk> ws_prog G; is_class G C\<rbrakk> \<Longrightarrow> 
+  ((method (comp G, C) S) = 
+  option_map (\<lambda> (D,rT,b).  (D, rT, mtd_mb (compMethod G D (S, rT, b))))
+             (method (G, C) S))"
 apply (simp add: method_def)
 apply (frule wf_subcls1)
 apply (simp add: comp_class_rec)
 apply (simp add: map_compose [THEN sym] split_iter split_compose del: map_compose)
-apply (rule_tac R="%x y. (x S) = Some (D, rT, mb) \<longrightarrow> (y S) = Some (D, rT, snd (snd (compMethod G D (S, rT, mb))))" in  class_rec_relation) apply assumption
+apply (rule_tac R="%x y. ((x S) = (option_map (\<lambda>(D, rT, b). 
+  (D, rT, snd (snd (compMethod G D (S, rT, b))))) (y S)))" 
+  in class_rec_relation)
+apply assumption
 
 apply (intro strip)
 apply simp
 
-apply (frule_tac f="(\<lambda>(s, m). (s, Object, m))" 
-  and g="(Fun.comp (\<lambda>(s, m). (s, Object, m)) (compMethod G Object))" in map_of_map_fst)
-(*
-apply (frule_tac f="(\<lambda>(s, m). (s, Object, m))" 
-  and g="((\<lambda>(s, m). (s, Object, m)) \<circ> compMethod G Object)" in map_of_map_fst)
-*)
-apply (simp add: inj_on_def)
+apply (rule trans)
+
+apply (rule_tac f="(\<lambda>(s, m). (s, Object, m))" and
+  g="(Fun.comp (\<lambda>(s, m). (s, Object, m)) (compMethod G Object))" 
+  in map_of_map_fst)
+defer				(* inj \<dots> *)
+apply (simp add: inj_on_def split_beta) 
 apply (simp add: split_beta compMethod_def)
-apply (simp add: split_beta compMethod_def)
+apply (simp add: map_of_map [THEN sym])
+apply (simp add: split_beta)
+apply (simp add: map_compose [THEN sym] Fun.comp_def split_beta)
+apply (subgoal_tac "(\<lambda>x\<Colon>(vname list \<times> fdecl list \<times> stmt \<times> expr) mdecl.
+                    (fst x, Object,
+                     snd (compMethod G Object
+                           (inv (\<lambda>(s\<Colon>sig, m\<Colon>ty \<times> vname list \<times> fdecl list \<times> stmt \<times> expr).
+                                    (s, Object, m))
+                             (S, Object, snd x)))))
+  = (\<lambda>x. (fst x, Object, fst (snd x),
+                        snd (snd (compMethod G Object (S, snd x)))))")
 apply (simp only:)
-apply (subgoal_tac "(inv (\<lambda>(s, m). (s, Object, m)) (S, D, rT, mb)) = (S, rT, mb)")
+apply (simp add: expand_fun_eq)
+apply (intro strip)
+apply (subgoal_tac "(inv (\<lambda>(s, m). (s, Object, m)) (S, Object, snd x)) = (S, snd x)")
 apply (simp only:)
 apply (simp add: compMethod_def split_beta)
-apply (simp add: map_of_map) apply (erule exE)+ apply simp
-apply (simp add: map_of_map) apply (erule exE)+ apply simp
-apply (rule inv_f_eq) apply (simp add: inj_on_def) apply simp
+apply (rule inv_f_eq) 
+defer
+defer
 
 apply (intro strip)
 apply (simp add: map_add_Some_iff map_of_map del: split_paired_Ex)
-apply (subgoal_tac "\<forall>x\<in>set ms. fst ((Fun.comp (\<lambda>(s, m). (s, Ca, m)) (compMethod G Ca)) x) = fst x")
-(*
-apply (subgoal_tac "\<forall>x\<in>set ms. fst (((\<lambda>(s, m). (s, Ca, m)) \<circ> compMethod G Ca) x) = fst x")
-*)
-apply (erule disjE)
-apply (rule disjI1)
-apply (simp add: map_of_map2)
-apply (simp (no_asm_simp) add: compMethod_def split_beta)
-
-apply (rule disjI2)
-apply (simp add: map_of_map2)
-
-  -- "subgoal"
-apply (simp (no_asm_simp) add: compMethod_def split_beta)
-
-apply (simp add: is_class_def)
-done
-
-
-constdefs comp_method_result :: "java_mb prog \<Rightarrow> sig \<Rightarrow> 
-  (cname \<times> ty \<times> java_mb) option \<Rightarrow> (cname \<times> ty \<times> jvm_method) option"
-  "comp_method_result G S m ==  case m of 
-    None \<Rightarrow> None
-  | Some (D, rT, mb) \<Rightarrow> Some (D, rT, mtd_mb (compMethod G D (S, rT, mb)))"
-
-
-lemma map_of_map_compMethod: "map_of (map (\<lambda>(s, m). (s, C, m)) (map (compMethod G C) ms)) S =
-          (case map_of (map (\<lambda>(s, m). (s, C, m)) ms) S of None \<Rightarrow> None
-           | Some (D, rT, mb) \<Rightarrow> Some (D, rT, mtd_mb (compMethod G D (S, rT, mb))))"
-apply (induct ms)
-apply simp
-apply (simp only: map_compose [THEN sym])
-apply (simp add: o_def split_beta del: map.simps)
-apply (simp (no_asm_simp) only: map.simps map_of.simps)
+apply (simp add: map_add_def)
+apply (subgoal_tac "inj (\<lambda>(s, m). (s, Ca, m))")
+apply (drule_tac g="(Fun.comp (\<lambda>(s, m). (s, Ca, m)) (compMethod G Ca))" and xs=ms
+  and k=S in map_of_map_fst) 
+apply (simp add: split_beta) 
 apply (simp add: compMethod_def split_beta)
+apply (case_tac "(map_of (map (\<lambda>(s, m). (s, Ca, m)) ms) S)")
+apply simp
+apply simp apply (simp add: split_beta map_of_map) apply (erule exE) apply (erule conjE)+
+apply (drule_tac t=a in sym)
+apply (subgoal_tac "(inv (\<lambda>(s, m). (s, Ca, m)) (S, a)) = (S, snd a)")
+apply simp
+apply (subgoal_tac "\<forall>x\<in>set ms. fst ((Fun.comp (\<lambda>(s, m). (s, Ca, m)) (compMethod G Ca)) x) = fst x")
+   prefer 2 apply (simp (no_asm_simp) add: compMethod_def split_beta)
+apply (simp add: map_of_map2)
+apply (simp (no_asm_simp) add: compMethod_def split_beta)
+
+  -- "remaining subgoals"
+apply (auto intro: inv_f_eq simp add: inj_on_def is_class_def)
 done
 
-  (* the following is more expressive than comp_method and should replace it *)
-lemma comp_method_eq [rule_format (no_asm)]: "wf_prog wf_mb G \<Longrightarrow> is_class G C \<longrightarrow>
-method (comp G, C) S = comp_method_result G S (method (G,C) S)"
-apply (subgoal_tac "wf ((subcls1 G)^-1)") prefer 2 apply (rule wf_subcls1, assumption) 
 
-apply (rule subcls_induct)
-apply assumption
-apply (intro strip)
-apply (subgoal_tac "\<exists> D fs ms. class G C = Some (D, fs, ms)") 
-   prefer 2 apply (simp add: is_class_def)
-apply (erule exE)+
 
-apply (case_tac "C = Object")
-
-  (* C = Object *)
-apply (subst method_rec_lemma) apply assumption+ apply simp 
-apply (subst method_rec_lemma) apply (frule comp_class_imp) apply assumption+ 
-   apply (simp add: comp_subcls1) 
-apply (simp add: comp_method_result_def)
-apply (rule map_of_map_compMethod) 
-
-  (* C \<noteq> Object *)
-apply (subgoal_tac "(C, D) \<in> (subcls1 G)\<^sup>+") 
-   prefer 2 apply (frule subcls1I, assumption+) apply blast
-apply (subgoal_tac "is_class G D")
-apply (drule spec, drule mp, assumption, drule mp, assumption)
-apply (frule wf_subcls1) 
-apply (subgoal_tac "wf ((subcls1 (comp G))\<inverse>)")
-apply (frule_tac G=G in method_rec_lemma, assumption)
-apply (frule comp_class_imp)
-apply (frule_tac G="comp G" in method_rec_lemma, assumption)
-apply (simp only:)
-apply (simp (no_asm_simp) add: comp_method_result_def expand_fun_eq)
-
-apply (case_tac "(method (G, D) ++  map_of (map (\<lambda>(s, m). (s, C, m)) ms)) S")
-
-  (* case None *)
-apply (simp (no_asm_simp) add: map_add_None)
-apply (simp add: map_of_map_compMethod comp_method_result_def) 
-
-  (* case Some *)
-apply (simp add: map_add_Some_iff)
-apply (erule disjE)
-  apply (simp add: split_beta map_of_map_compMethod)
-  apply (simp add: map_add_def comp_method_result_def map_of_map_compMethod)
-
-  (* show subgoals *)
-apply (simp add: comp_subcls1) 
-  (* show is_class G D *)
-apply (simp add: wf_prog_def wf_cdecl_def)
-apply (subgoal_tac "(C, D, fs, ms)\<in>set G")
-apply blast
-apply (simp add: class_def map_of_SomeD)
-done
-
-  (* ### this proof is horrid and has to be redone *)
-lemma unique_map_fst [rule_format]: "(\<forall> x \<in> set xs. (fst x = fst (f x) )) \<longrightarrow>
-  unique xs = unique (map f xs)"
-apply (induct_tac "xs")
-apply simp
-apply (intro strip)
-apply simp
-apply (case_tac a, simp)
-apply (case_tac "f (aa, b)")
-apply (simp only:)
-apply (simp only: unique_Cons)
-
-apply simp
-apply (subgoal_tac "(\<exists>y. (ab, y) \<in> set list) = (\<exists>y. (ab, y) \<in> f ` set list)")
-apply blast
+lemma comp_wf_mrT: "\<lbrakk> ws_prog G; is_class G D\<rbrakk> \<Longrightarrow> 
+  wf_mrT (TranslComp.comp G) (C, D, fs, map (compMethod G a) ms) =
+  wf_mrT G (C, D, fs, ms)"
+apply (simp add: wf_mrT_def compMethod_def split_beta)
+apply (simp add: comp_widen)
 apply (rule iffI)
-
-apply clarify
-apply (rule_tac x="(snd (f(ab, y)))" in exI)
+apply (intro strip)
 apply simp
-apply (subgoal_tac "(ab, snd (f (ab, y))) = (fst (f (ab, y)), snd (f (ab, y)))")
-apply (simp only:)
-apply (simp add: surjective_pairing [THEN sym])
-apply (subgoal_tac "fst (f (ab, y)) = fst (ab, y)")
-apply simp
-apply (drule bspec) apply assumption apply simp
-
-apply clarify
-apply (drule bspec) apply assumption apply simp
-apply (subgoal_tac "ac = ab")
-apply simp
-apply blast
-apply (drule sym)
-apply (drule sym)
-apply (drule_tac f=fst in arg_cong)
-apply simp
-done
-
-lemma comp_unique: "unique G = unique (comp G)"
-apply (simp add: comp_def)
-apply (rule unique_map_fst)
-apply (simp add: compClass_def split_beta)
+apply (drule bspec) apply assumption
+apply (drule_tac x=D' in spec) apply (drule_tac x=rT' in spec) apply (drule mp)
+prefer 2 apply assumption
+apply (simp add: comp_method [of G D])
+apply (erule exE)+
+apply (subgoal_tac "z =(fst z, fst (snd z), snd (snd z))")
+apply (rule exI)
+apply (simp)
+apply (simp add: split_paired_all)
+apply (intro strip)
+apply (simp add: comp_method)
+apply auto
 done
 
 
@@ -396,9 +388,6 @@ done
   (* DIVERSE OTHER LEMMAS *)
 (**********************************************************************)
 
-
-(* already proved less elegantly in CorrComp.thy;
-  to be moved into a common super-theory *)
 lemma max_spec_preserves_length:
   "max_spec G C (mn, pTs) = {((md,rT),pTs')} 
   \<Longrightarrow> length pTs = length pTs'"
@@ -408,7 +397,6 @@ apply (simp add: list_all2_def)
 done
 
 
-(* already proved in CorrComp.thy \<longrightarrow> into common supertheory *)
 lemma ty_exprs_length [simp]: "(E\<turnstile>es[::]Ts \<longrightarrow> length es = length Ts)"
 apply (subgoal_tac "(E\<turnstile>e::T \<longrightarrow> True) \<and> (E\<turnstile>es[::]Ts \<longrightarrow> length es = length Ts) \<and> (E\<turnstile>s\<surd> \<longrightarrow> True)")
 apply blast
@@ -425,5 +413,13 @@ apply (erule exE)+
 apply (simp add: method_rT_def)
 done
 
+  (**********************************************************************************)
+
+declare compClass_fst [simp del]
+declare compClass_fst_snd [simp del]
+declare compClass_fst_snd_snd [simp del]
+
+declare split_paired_All [simp add]
+declare split_paired_Ex [simp add]
 
 end
